ocaml/src/ConfigUtil.ml
@@ -112,6 +112,7 @@ type eval_config =
     { debug : bool ref;
       eval_only : bool ref;
       mutable eval_io : Data.json option;
+      mutable eval_schema : string option;
       mutable format : serialization_format;
       mutable eval_inputs : string list;
       eval_lang_config : lang_config }
@@ -120,11 +121,13 @@ let default_eval_config () =
   { debug = ref false;
     eval_only = ref false;
     eval_io = None;
+    eval_schema = None;
     format = META;
     eval_inputs = [];
     eval_lang_config = default_eval_lang_config () }
 
 let set_eval_io conf io = conf.eval_io <- Some io
+let set_eval_schema conf schema = conf.eval_schema <- Some schema
 let set_input conf f = conf.eval_inputs <- f :: conf.eval_inputs
 
 let set_format conf s =
@@ -138,6 +141,7 @@ let get_eval_lang_config conf = conf.eval_lang_config
 let get_eval_only conf = conf.eval_only
 let get_debug conf = conf.debug
 let get_eval_io conf = conf.eval_io
+let get_eval_schema conf = conf.eval_schema
 let get_eval_inputs conf = conf.eval_inputs
 
 (* Data Section *)
